To change the logarithmic equation \( y = -\log_3(x - 1) \) to its exponential form, we'll go through the process step by step:

### Step 1: Rewrite the Equation

Start with the given equation:
\[ y = -\log_3(x - 1) \]

### Step 2: Isolate the Logarithm

To isolate the logarithmic part, multiply both sides by -1:
\[ -y = \log_3(x - 1) \]

### Step 3: Convert Logarithmic Form to Exponential Form

Recall that the logarithmic equation \( \log_b(a) = c \) is equivalent to the exponential equation \( b^c = a \).

In this case:

- The base \( b \) is 3.
- The exponent \( c \) is \(-y\).
- The result \( a \) is \(x - 1\).

So, converting the logarithmic equation to exponential form gives:
\[ 3^{-y} = x - 1 \]

### Step 4: Solve for \(x\)

Now, solve for \(x\) by adding 1 to both sides:
\[ x = 3^{-y} + 1 \]

### Final Result:

The exponential form of the equation is:
\[ x = 3^{-y} + 1 \]

or
\[ x = \frac{1}{3y} + 1 \]

This is the exponential equivalent of the original logarithmic equation \( y = -\log_3(x - 1) \).
